More syntax, other cosmetics

Scratchpad/LTree.thy
@@ -2,33 +2,33 @@ theory LTree
 imports Main  "$AFP/Coinductive/Coinductive_List"
 begin
 
-codatatype (lset: 'a) ltree = Node (lnext : "'a \<Rightarrow> 'a ltree option")
+codatatype (lset: 'a) tree = Node (nxt : "'a \<Rightarrow> 'a tree option")
 
-primcorec lempty :: "'a ltree"
-  where "lnext lempty = (\<lambda> _ . None)"
+primcorec empty :: "'a tree"
+  where "nxt empty = (\<lambda> _ . None)"
 
-primcorec single :: "'a \<Rightarrow> 'a ltree"
-  where "lnext (single x) = (\<lambda> _ . None)(x := Some lempty)"
+primcorec single :: "'a \<Rightarrow> 'a tree"
+  where "nxt (single x) = (\<lambda> _ . None)(x := Some empty)"
 
-primcorec many :: "'a \<Rightarrow> 'a ltree"
-  where "lnext (many x) = (\<lambda> x'. if x' = x then Some (many x) else None)"
+primcorec many :: "'a \<Rightarrow> 'a tree"
+  where "nxt (many x) = (\<lambda> x'. if x' = x then Some (many x) else None)"
 
-primcorec lanything :: "'a ltree"
-  where "lnext lanything = (\<lambda> _ . Some lanything)"
+primcorec anything :: "'a tree"
+  where "nxt anything = (\<lambda> _ . Some anything)"
 
-coinductive lpaths_aux :: "'a ltree \<Rightarrow> 'a llist \<Rightarrow> bool"
-  where "lpaths_aux t LNil"
-      | "lnext t x = Some t' \<Longrightarrow> lpaths_aux t' l \<Longrightarrow> lpaths_aux t (LCons x l)"
+coinductive paths_aux :: "'a tree \<Rightarrow> 'a llist \<Rightarrow> bool"
+  where "paths_aux t LNil"
+      | "nxt t x = Some t' \<Longrightarrow> paths_aux t' l \<Longrightarrow> paths_aux t (LCons x l)"
 
-definition lpaths :: "'a ltree \<Rightarrow> 'a llist set" 
-  where "lpaths t = Collect (lpaths_aux t)"
-lemma elim_lpaths_aux[pred_set_conv]: "lpaths_aux t p \<longleftrightarrow> p \<in> lpaths t" unfolding lpaths_def by simp
-lemmas lpaths_intros[intro?] = lpaths_aux.intros[unfolded elim_lpaths_aux]
-lemmas lpaths_coinduct[consumes 1, coinduct set: lpaths] = lpaths_aux.coinduct[to_set]
-lemmas lpaths_cases[consumes 1, cases set: lpaths] = lpaths_aux.cases[to_set]
-lemmas lpaths_simpss = lpaths_aux.simps[to_set]
+definition paths :: "'a tree \<Rightarrow> 'a llist set" 
+  where "paths t = Collect (paths_aux t)"
+lemma elim_paths_aux[pred_set_conv]: "paths_aux t p \<longleftrightarrow> p \<in> paths t" unfolding paths_def by simp
+lemmas paths_intros[intro?] = paths_aux.intros[unfolded elim_paths_aux]
+lemmas paths_coinduct[consumes 1, coinduct set: paths] = paths_aux.coinduct[to_set]
+lemmas paths_cases[consumes 1, cases set: paths] = paths_aux.cases[to_set]
+lemmas paths_simpss = paths_aux.simps[to_set]
 
-lemma "repeat x \<in> lpaths (many x)"
+lemma "repeat x \<in> paths (many x)"
   apply (coinduction)
   apply (rule disjI2)
   apply auto
@@ -43,38 +43,35 @@ fun op_option :: "('a \<Rightarrow> 'a \<Rightarrow> 'a) \<Rightarrow> 'a option
       | "op_option f None     (Some y) = Some y"
       | "op_option f None     None     = None"
 (*
-primcorec lor :: "'a ltree \<Rightarrow> 'a ltree \<Rightarrow> 'a ltree"
-  where "lnext (lor t1 t2) = (\<lambda> x. op_option lor (lnext t1 x) (lnext t2 x))"
+primcorec or :: "'a tree \<Rightarrow> 'a tree \<Rightarrow> 'a tree"
+  where "nxt (or t1 t2) = (\<lambda> x. op_option or (nxt t1 x) (nxt t2 x))"
 *)
-primcorec lor :: "'a ltree \<Rightarrow> 'a ltree \<Rightarrow> 'a ltree"
-  where "lnext (lor t1 t2) = (\<lambda> x.
-           case (lnext t1 x) of Some t1' \<Rightarrow> (case lnext t2 x of Some t2' \<Rightarrow> Some (lor t1' t2') | None \<Rightarrow> Some t1')
-                              | None     \<Rightarrow> lnext t2 x)"
+primcorec or :: "'a tree \<Rightarrow> 'a tree \<Rightarrow> 'a tree"
+  where "nxt (or t1 t2) = (\<lambda> x.
+           case (nxt t1 x) of Some t1' \<Rightarrow> (case nxt t2 x of Some t2' \<Rightarrow> Some (or t1' t2') | None \<Rightarrow> Some t1')
+                              | None     \<Rightarrow> nxt t2 x)"
 
-lemma lor_simp:  "lnext (lor t1 t2) x =  op_option lor (lnext t1 x) (lnext t2 x)"
-  by (cases "lnext t1 x", case_tac [!] "lnext t2 x") auto
-
-
-primcorec land_aux :: "'a ltree \<Rightarrow> 'a ltree \<Rightarrow> 'a ltree"
-      and land :: "'a ltree \<Rightarrow> 'a ltree \<Rightarrow> 'a ltree"
-  where "(land_aux t1 t2) = Node (\<lambda> x. case (lnext t1 x) of Some t1' \<Rightarrow> Some (land t1' t2) | None \<Rightarrow> None)"
-       |"(land t1 t2) = lor (land_aux t1 t2) (land_aux t2 t1)"
-
+lemma or_simp:  "nxt (or t1 t2) x =  op_option or (nxt t1 x) (nxt t2 x)"
+  by (cases "nxt t1 x", case_tac [!] "nxt t2 x") auto
 
 (*
-primcorec land :: "'a ltree \<Rightarrow> 'a ltree \<Rightarrow> 'a ltree"
-   where "(land t1 t2) = lor (Node (\<lambda> x. case (lnext t1 x) of Some t1' \<Rightarrow> Some (land t1' t2) | None \<Rightarrow> None)) (Node (\<lambda> x. case (lnext t1 x) of Some t1' \<Rightarrow> Some (land t1' t2) | None \<Rightarrow> None))"
+primcorec and_aux :: "'a tree \<Rightarrow> 'a tree \<Rightarrow> 'a tree"
+      and and :: "'a tree \<Rightarrow> 'a tree \<Rightarrow> 'a tree"
+  where "(and_aux t1 t2) = Node (\<lambda> x. case (nxt t1 x) of Some t1' \<Rightarrow> Some (and t1' t2) | None \<Rightarrow> None)"
+       |"(and t1 t2) = or (and_aux t1 t2) (and_aux t2 t1)"
+
+primcorec and :: "'a tree \<Rightarrow> 'a tree \<Rightarrow> 'a tree"
+   where "(and t1 t2) = or (Node (\<lambda> x. case (nxt t1 x) of Some t1' \<Rightarrow> Some (and t1' t2) | None \<Rightarrow> None)) (Node (\<lambda> x. case (nxt t1 x) of Some t1' \<Rightarrow> Some (and t1' t2) | None \<Rightarrow> None))"
+
+primcorec and :: "'a tree \<Rightarrow> 'a tree \<Rightarrow> 'a tree"
+   where "nxt (and t1 t2) = (\<lambda> x.
+      case (nxt t1 x) of Some t1' \<Rightarrow> (case nxt t2 x of Some t2' \<Rightarrow> Some (or (and t1' t2) (and t1 t2')) | None \<Rightarrow> Some (and t1' t2))
+                         | None     \<Rightarrow> (case nxt t2 x of Some t2' \<Rightarrow> Some (and t1 t2')                     | None \<Rightarrow> None))"
+
+primcorec and :: "'a tree \<Rightarrow> 'a tree \<Rightarrow> 'a tree"
+   where "nxt (and t1 t2) = map_option (\<lambda> (x,y). (and x y, and x y)) o (\<lambda> x.
+      case (nxt t1 x) of Some t1' \<Rightarrow> (case nxt t2 x of Some t2' \<Rightarrow> Some (or t1' t1, or t2 t2') | None \<Rightarrow> Some (t1', t2))
+                         | None     \<Rightarrow> (case nxt t2 x of Some t2' \<Rightarrow> Some (t1, t2')                | None \<Rightarrow> None))"
 *)
-
-primcorec land :: "'a ltree \<Rightarrow> 'a ltree \<Rightarrow> 'a ltree"
-   where "lnext (land t1 t2) = (\<lambda> x.
-      case (lnext t1 x) of Some t1' \<Rightarrow> (case lnext t2 x of Some t2' \<Rightarrow> Some (lor (land t1' t2) (land t1 t2')) | None \<Rightarrow> Some (land t1' t2))
-                         | None     \<Rightarrow> (case lnext t2 x of Some t2' \<Rightarrow> Some (land t1 t2')                     | None \<Rightarrow> None))"
-
-primcorec land :: "'a ltree \<Rightarrow> 'a ltree \<Rightarrow> 'a ltree"
-   where "lnext (land t1 t2) = map_option (\<lambda> (x,y). (land x y, land x y)) o (\<lambda> x.
-      case (lnext t1 x) of Some t1' \<Rightarrow> (case lnext t2 x of Some t2' \<Rightarrow> Some (lor t1' t1, lor t2 t2') | None \<Rightarrow> Some (t1', t2))
-                         | None     \<Rightarrow> (case lnext t2 x of Some t2' \<Rightarrow> Some (t1, t2')                | None \<Rightarrow> None))"
-
 
 end
