Launchbury/Denotational.thy
@@ -8,7 +8,9 @@ This is the actual denotational semantics as found in \cite{launchbury}.
 
 interpretation semantic_domain Fn Fn_project B B_project "(\<Lambda> x. x)".
 
-abbreviation ESem_syn'' ("\<lbrakk> _ \<rbrakk>\<^bsub>_\<^esub>"  [60,60] 60) where "\<lbrakk> e \<rbrakk>\<^bsub>\<rho>\<^esub> \<equiv> ESem e \<cdot> \<rho>"
+abbreviation ESem_syn'' :: "exp \<Rightarrow> (var => Value) \<Rightarrow> Value" ("\<lbrakk> _ \<rbrakk>\<^bsub>_\<^esub>"  [60,60] 60)
+  where "\<lbrakk> e \<rbrakk>\<^bsub>\<rho>\<^esub> \<equiv> ESem e \<cdot> \<rho>"
+
 abbreviation EvalHeapSem_syn''  ("\<^bold>\<lbrakk> _ \<^bold>\<rbrakk>\<^bsub>_\<^esub>"  [0,0] 110)  where "\<^bold>\<lbrakk>\<Gamma>\<^bold>\<rbrakk>\<^bsub>\<rho>\<^esub> \<equiv> evalHeap \<Gamma> (\<lambda> e. \<lbrakk>e\<rbrakk>\<^bsub>\<rho>\<^esub>)"
 abbreviation HSem_syn' ("\<lbrace>_\<rbrace>_"  [60,60] 60) where "\<lbrace>\<Gamma>\<rbrace>\<rho> \<equiv> HSem \<Gamma> \<cdot> \<rho>"
 abbreviation HSem_bot  ("\<lbrace>_\<rbrace>"  [60] 60) where "\<lbrace>\<Gamma>\<rbrace> \<equiv> \<lbrace>\<Gamma>\<rbrace>\<bottom>"
@@ -21,6 +23,7 @@ lemma ESem_simps_as_defined:
   "\<lbrakk> (scrut ? e\<^sub>1 : e\<^sub>2) \<rbrakk>\<^bsub>\<rho>\<^esub> = B_project\<cdot>(\<lbrakk> scrut \<rbrakk>\<^bsub>\<rho>\<^esub>)\<cdot>(\<lbrakk> e\<^sub>1 \<rbrakk>\<^bsub>\<rho>\<^esub>)\<cdot>(\<lbrakk> e\<^sub>2 \<rbrakk>\<^bsub>\<rho>\<^esub>)"
   "\<lbrakk> Let \<Gamma> body \<rbrakk>\<^bsub>\<rho>\<^esub> = \<lbrakk>body\<rbrakk>\<^bsub>\<lbrace>\<Gamma>\<rbrace>(\<rho> f|` fv (Let \<Gamma> body))\<^esub>"
   by (simp_all del: ESem_Lam ESem_Let add: ESem.simps(1,4) )
+
 
 lemma ESem_simps:
   "\<lbrakk> Lam [x]. e \<rbrakk>\<^bsub>\<rho>\<^esub> =  Fn\<cdot>(\<Lambda> v. \<lbrakk> e \<rbrakk>\<^bsub>\<rho>(x := v)\<^esub>)"
