ROOT
@@ -10,6 +10,12 @@ session DissFiles = "HOLCF-Nominal2" +
     "Call_Arity/ArityAnalysisCorrDenotational"
   document_files "root.tex"
 
+session DissExtraFiles = "HOLCF-Nominal2" +
+  options [document = pdf, document_output = "/home/jojo/uni/diss/isa-thy-output"]
+  theories
+    "Scratchpad/ITree"
+    "Scratchpad/LTree"
+  document_files "root.tex"
 
 
 session Arity (AFP) in "Call_Arity" = "HOLCF-Nominal2" +
@@ -27,3 +33,18 @@ session Arity (AFP) in "Call_Arity" = "HOLCF-Nominal2" +
     "NoCardinalityAnalysis"
     "CallArityEnd2EndSafe"
     "ArityAnalysisCorrDenotational"
+
+
+session Call_Arity_Paperstats (AFP) = "HOLCF-Nominal2" +
+  options [document = pdf, document_output = "/tmp/call-arity-paperstats"]
+  theories
+    (* "Call_Arity/SestoftCorrect" *)
+    "Call_Arity/TrivialArityAnal"
+    "Call_Arity/NoCardinalityAnalysis"
+    "Call_Arity/ArityTransformSafe"
+    "Call_Arity/CallArityEnd2EndSafe"
+    "Call_Arity/ArityAnalysisCorrDenotational"
+  document_files
+    "root.tex"
+
+
